Test/civl/samples/TryIncNBelowMax.bpl
@@ -5,7 +5,7 @@ var {:layer 0, 2} count: int;
 const max: int;
 
 yield procedure {:layer 1} TryIncBelowMax() returns (ok: bool)
-requires call Yield1();
+preserves call Yield1();
 refines atomic action {:layer 2} _ {
     if (ok) {
         assume count < max;
@@ -13,15 +13,16 @@ refines atomic action {:layer 2} _ {
     }
 }
 {
-    var retry_limit: int;
+    var limit: int;
 
-    call retry_limit := ComputeLimit() | Yield1();
-    async call backgroundMaintenance();
-    call ok := HelperInc(0, retry_limit);
+    call limit := ComputeLimit() | Yield1();
+    assert {:layer 1} limit >= 0;
+    async call BackgroundMaintenance();
+    call ok := HelperInc(0, limit);
 }
 
-yield procedure {:layer 1} HelperInc(tries: int, retry_limit: int) returns (ok: bool)
-requires call Yield1();
+yield procedure {:layer 1} HelperInc(tries: int, limit: int) returns (ok: bool)
+preserves call Yield1();
 refines atomic action {:layer 2} _ {
     if (ok) {
         assume count < max;
@@ -31,17 +32,15 @@ refines atomic action {:layer 2} _ {
 {
     var n: int;
 
-    if (tries > retry_limit) {
-        ok := false; // retry limit reached
-        return; 
+    if (tries >= limit) {
+        ok := false; // limit reached
+        return;
     }
-
-    call Yield1();
 
     call n := Read();
     if (n >= max) {
         ok := false; 
-        return; 
+        return;
     }
 
     call Yield1();
@@ -50,19 +49,15 @@ refines atomic action {:layer 2} _ {
     if (ok) {
         return;
     }
-    call ok := HelperInc(tries+1, retry_limit);
+    call ok := HelperInc(tries+1, limit);
+    assert {:layer 1} count <= max;
 }
 
-yield procedure {:layer 1} ComputeLimit() returns (retry_limit: int)
-refines atomic action {:layer 2} _ {
-    assume retry_limit > 0;
-}
-{
-    assume retry_limit > 0;
-}
+yield procedure {:layer 1} ComputeLimit() returns (limit: int);
+refines atomic action {:layer 2} _ { }
+ensures {:layer 1} limit >= 0;
 
-
-yield procedure {:layer 1} backgroundMaintenance() 
+yield procedure {:layer 1} BackgroundMaintenance()
 preserves call Yield1();
 {
     assert {:layer 1} count <= max; 
